backend/LTL.v
@@ -106,6 +106,17 @@ Definition return_regs (caller callee: locset) : locset :=
     | S sl ofs ty => caller (S sl ofs ty)
     end.
 
+(** [undef_caller_save_regs ls] models the effect of calling
+    an external function: caller-save registers can change unpredictably,
+    hence we set them to [Vundef]. *)
+
+Definition undef_caller_save_regs (ls: locset) : locset :=
+  fun (l: loc) =>
+    match l with
+    | R r => if is_callee_save r then ls (R r) else Vundef
+    | S sl ofs ty => ls (S sl ofs ty)
+    end.
+
 (** LTL execution states. *)
 
 Inductive stackframe : Type :=
@@ -259,7 +270,7 @@ Inductive step: state -> trace -> state -> Prop :=
   | exec_function_external: forall s ef t args res rs m rs' m',
       args = map (fun p => Locmap.getpair p rs) (loc_arguments (ef_sig ef)) ->
       external_call ef ge args m t res m' ->
-      rs' = Locmap.setpair (loc_result (ef_sig ef)) res rs ->
+      rs' = Locmap.setpair (loc_result (ef_sig ef)) res (undef_caller_save_regs rs) ->
       step (Callstate s (External ef) rs m)
          t (Returnstate s rs' m')
   | exec_return: forall f sp rs1 bb s rs m,
