riscV/Asm.v
@@ -1013,6 +1013,15 @@ Definition preg_of (r: mreg) : preg :=
   | Machregs.F28 => F28 | Machregs.F29 => F29 | Machregs.F30 => F30 | Machregs.F31 => F31
   end.
 
+(** Undefine all registers except SP and callee-save registers *)
+
+Definition undef_caller_save_regs (rs: regset) : regset :=
+  fun r =>
+    if preg_eq r SP
+    || In_dec preg_eq r (List.map preg_of (List.filter is_callee_save all_mregs))
+    then rs r
+    else Vundef.
+
 (** Extract the values of the arguments of an external call.
     We exploit the calling conventions from module [Conventions], except that
     we use RISC-V registers instead of locations. *)
@@ -1073,7 +1082,7 @@ Inductive step: state -> trace -> state -> Prop :=
       Genv.find_funct_ptr ge b = Some (External ef) ->
       external_call ef ge args m t res m' ->
       extcall_arguments rs m (ef_sig ef) args ->
-      rs' = (set_pair (loc_external_result (ef_sig ef) ) res rs)#PC <- (rs RA) ->
+      rs' = (set_pair (loc_external_result (ef_sig ef) ) res (undef_caller_save_regs rs))#PC <- (rs RA) ->
       step (State rs m) t (State rs' m').
 
 End RELSEM.
